src/Std/Data/TreeMap/Basic.lean
@@ -81,6 +81,10 @@ def insert (l : TreeMap α β cmp) (a : α) (b : β) : TreeMap α β cmp :=
 def contains (l : TreeMap α β cmp) (a : α) : Bool :=
   l.inner.contains a
 
+@[inline, inherit_doc DTreeMap.erase]
+def erase (l : TreeMap α β cmp) (a : α) : TreeMap α β cmp :=
+  ⟨l.inner.erase a⟩
+
 instance : Membership α (TreeMap α β cmp) where
   mem m a := m.contains a
 
