src/Std/Data/TreeSet/Raw.lean
@@ -123,6 +123,11 @@ Observe that this is different behavior than for lists: for lists, `∈` uses `=
 def contains (l : Raw α cmp) (a : α) : Bool :=
   l.inner.contains a
 
+/-- Removes the given key if it exists. -/
+@[inline]
+def erase (l : Raw α cmp) (a : α) : Raw α cmp :=
+  ⟨l.inner.erase a⟩
+
 instance : Membership α (Raw α cmp) where
   mem m a := m.contains a
 
