src/Std/Data/DTreeMap/Internal/Impl.lean
@@ -41,6 +41,8 @@ inductive WF [Ord α] : Impl α β → Prop where
   | empty : WF .empty
   /-- `insert` preserves well-formedness. Later shown to be subsumed by `.wf`. -/
   | insert {t h k v} : WF t → WF (t.insert k v h).impl
+  /-- `erase` preserves well-formedness. Later shown to be subsumed by `.wf`. -/
+  | erase {t h k} : WF t → WF (t.erase k h).impl
 
 /-- A well-formed tree is balanced. This is needed here already because we need to know that the
 tree is balanced to call the optimized modification functions. -/
@@ -48,6 +50,7 @@ theorem WF.balanced [Ord α] {t : Impl α β} : WF t → t.Balanced
   | .wf h _ => h
   | .empty => balanced_empty
   | .insert _ => TreeB.balanced_impl _
+  | .erase _ => TreeB.balanced_impl _
 
 end Impl
 
